src/go_lang/lifting.v
@@ -361,6 +361,68 @@ Proof.
   iModIntro. iSplit=>//. iSplit; first done. iFrame. by iApply "HΦ".
 Qed.
 
+Theorem MapGetS' l k vs m_def σ :
+     σ.(heap) !! l = Some vs ->
+     map_val vs = Some m_def ->
+     head_step (MapGet (Val $ LitV $ LitLoc l) (Val $ LitV $ LitInt $ k)) σ
+               []
+               (Val $ PairV (fst (map_get m_def k)) (LitV $ LitBool (snd (map_get m_def k)))) σ
+               [].
+Proof.
+  intros.
+  destruct_with_eqn (map_get m_def k).
+  eapply MapGetS; eauto.
+Qed.
+
+Hint Resolve MapGetS' : core.
+
+Definition map_mapsto l q m_def :=
+  (∃ vs, l ↦{q} vs ∗ ⌜ map_val vs = Some m_def ⌝)%I.
+
+Lemma wp_map_get s E l q m_def k :
+  {{{ ▷ map_mapsto l q m_def }}} MapGet (Val $ LitV (LitLoc l)) (Val $ LitV $ LitInt k) @ s; E
+  {{{ r ok, RET PairV r (LitV $ LitBool ok); ⌜ map_get m_def k = (r, ok) ⌝ ∗ map_mapsto l q m_def }}}.
+Proof.
+  iIntros (Φ) ">Hl HΦ".
+  iDestruct "Hl" as (vs) "(Hl&Hmap)".
+  iDestruct "Hmap" as %Hmap.
+  iApply wp_lift_atomic_head_step_no_fork; auto.
+  iIntros (σ1 κ κs n) "[Hσ Hκs] !>". iDestruct (@gen_heap_valid with "Hσ Hl") as %?.
+  iSplit.
+  { iPureIntro.
+    eexists _, _, _, _; simpl.
+    eapply MapGetS'; eauto. }
+  iNext; iIntros (v2 σ2 efs Hstep); inv_head_step.
+  iModIntro. iSplit=>//. iFrame. iApply "HΦ".
+  iSplit; first by eauto.
+  iExists vs; by iFrame.
+Qed.
+
+Theorem map_cons_insert k v vs m_def :
+  map_val vs = Some m_def ->
+  map_val (MapConsV k v vs) = Some (map_insert m_def k v).
+Proof.
+  destruct m_def; simpl.
+  by intros ->.
+Qed.
+
+Lemma wp_map_insert s E l m_def k v :
+  {{{ ▷ map_mapsto l 1 m_def }}} MapInsert (Val $ LitV (LitLoc l)) (Val $ LitV $ LitInt k) (Val v) @ s; E
+  {{{ RET LitV LitUnit; map_mapsto l 1 (map_insert m_def k v) }}}.
+Proof.
+  iIntros (Φ) ">Hl HΦ".
+  iDestruct "Hl" as (vs) "(Hl&Hmap)".
+  iDestruct "Hmap" as %Hmap.
+  iApply wp_lift_atomic_head_step_no_fork; auto.
+  iIntros (σ1 κ κs n) "[Hσ Hκs] !>". iDestruct (@gen_heap_valid with "Hσ Hl") as %?.
+  iSplit; first by eauto.
+  iNext; iIntros (v2 σ2 efs Hstep); inv_head_step.
+  iMod (@gen_heap_update with "Hσ Hl") as "[$ Hl]".
+  iModIntro. iSplit=>//. iFrame. iApply "HΦ".
+  iExists _; iFrame.
+  erewrite map_cons_insert by eauto; auto.
+Qed.
+
 Lemma wp_cmpxchg_fail s E l q v' v1 v2 :
   v' ≠ v1 → vals_compare_safe v' v1 →
   {{{ ▷ l ↦{q} v' }}} CmpXchg (Val $ LitV $ LitLoc l) (Val v1) (Val v2) @ s; E
